ParserTactics.v
@@ -1,6 +1,10 @@
 Require Import Derivation.
 Require Import Grammar.
 Require Import List.
+Require Import MSets.
+Require Import ParserUtils.
+Require Import ParseTable.
+Require Import String.
 Import ListNotations.
 
 Ltac inv H := inversion H; clear H; subst.
@@ -8,7 +12,7 @@ Ltac inv H := inversion H; clear H; subst.
 (* Add this to crush *)
 Ltac solveNotFalse := simpl; unfold not; intros; inversion H. 
 
-Ltac crush :=
+Ltac derCrush :=
   repeat match goal with
          | |- _ /\ _ => split
          | |- In _ _ => repeat (try (left ; reflexivity) ; right)
@@ -24,4 +28,95 @@ Ltac crush :=
          | |- derivesList2 [] _  => apply derivesNil2
          | |- ?P = ?P => reflexivity
          | |- _ => simpl in *
+         end.
+
+Ltac crush :=
+  repeat match goal with
+           
+         | |- ?X = ?X => reflexivity
+
+         (* contradictions *)
+                           
+         | H : [] = _ ++ (_ :: _) |- _ =>
+           apply app_cons_not_nil in H
+                                       
+         | H : false = true |- _ => inv H
+                                        
+         | H : False |- _ => inv H
+
+         | H : isNT (T _) = true |- _ => inv H
+
+         | H : isT (NT _) = true |- _ => inv H
+
+         | H : firstGamma _ [] _ |- _ => inv H
+
+         | H : ?X <> ?X |- _ =>
+           exfalso; apply H; reflexivity
+
+         | H : InA _ _ [] |- _ => inv H
+
+         (* unpacking assumptions *)
+
+         | H : (_ :: _) = (_ :: _) |- _ =>
+           idtac "inv eq lists" ; inv H
+
+         | H : pair (NT _) _ = pair _  _ |- _ =>
+           idtac "inv eq pairs" ; inv H
+
+         | H : firstSym ?NT ?T |- SymbolSet.In ?T _ =>
+           idtac "firstSym |- SymbolSet.In";
+           inv H
+
+         | H : SymbolMap.Raw.PX.MapsTo _ _ _ |- _ =>
+           inv H
+
+         | H : SymbolMap.Raw.PX.eqke _ _ |- _ =>
+           inv H
+
+         | H : fst _ = fst _ |- _ =>
+           simpl in H; subst
+
+         | H : snd _ = snd _ |- _ =>
+           simpl in H; subst
+
+         | H : SymbolMap.find (NT (String _ _)) _ = Some _
+           |- _ => inv H
+
+         | H : firstGamma _ (_::_) _ |- _ =>
+           idtac "inv firstGamma" ; inv H
+
+         | H : In (_, _) _ |- _ =>
+           idtac "inv pair in list" ; destruct H
+
+         | H : SymbolSet.In _ _ |- _ => inv H
+
+         | H : InA _ _ (_::_) |- _ => inv H
+
+         | H : _ = SymbolSet.this _ |- _ => inv H
+                                 
+         (* lists, maps, and sets *)
+                  
+         | |- SymbolMap.find _ _ = Some _ =>
+           idtac "SymbolMap.find = Some";
+           unfold SymbolMap.find; reflexivity
+                                    
+         | |- In _ _ =>
+           idtac "List.In";
+           repeat (try (left; reflexivity); right)
+
+         | |- SymbolSet.In (T (String _ _)) _ =>
+           idtac "SymbolSet.In T";
+           repeat (try (apply InA_cons_hd; reflexivity);
+                   apply InA_cons_tl)
+
+         | |- SymbolSet.In (NT (String _ _)) _ =>
+           idtac "SymbolSet.In NT";
+           repeat (try (apply InA_cons_hd; reflexivity);
+                   apply InA_cons_tl)
+
+         (* simplifying goals *)
+                  
+         | |- SymbolMap.find _ _ = Some _  /\ SymbolSet.In _ _ =>
+           split 
+
          end.
